Updates to MLS.fsti

fstar/new/MLS.fsti
@@ -13,32 +13,60 @@ let bytes = MLS.Lib.Array.array Lib.IntTypes.uint8
 let group_message = group_id & bytes
 let welcome_message = participant_id & bytes
 
-// JP: any further changes?
 let entropy = bytes
+
+val key_package: Type0
 
 noeq
 type public_info = {
-  public_key: bytes;
+  key_package: key_package;
   user_id: participant_id;
 }
 
 noeq
 type private_info = {
   private_key: bytes;
-  user_id: participant_id;
 }
 
+noeq
+type credentials = {
+  signing_key: bytes;
+  identity: string;
+}
+
+// Assume here that the directory has generated a signing key for us; that our
+// public signing key is published somewhere in the directory; and that the
+// client of this code passes us both our own participant_id and our own private
+// signing key.
+//   The application takes care of maintaining a mapping of e.g. hash of a key
+// package to private key to be retrieved later if we are ever to receive a
+// welcome message encoded with these credentials.
+val fresh_key_package: entropy -> credentials -> key_package & private_key:bytes
+
 // TODO: expose a way to inject e.g. a uint32 into a group_id
-val create: entropy → private_info → g:group_id -> state g
+// Note that after we've created the group, we receive our freshly-assigned
+// participant id.
+val create: entropy → private_info → g:group_id -> state g & participant_id
 
-val add: #g:group_id -> state g → public_info → group_message & welcome_message
+// Internally, a new `participant_id` is assigned to the freshly-added user.
+// Provided the server does not reject the message, the application can extend
+// its mapping from the welcome message's participant_id to the corresponding
+// username and endpoint.
+val add: #g:group_id -> state g → key_package → group_message & welcome_message
 
-val remove: #g:group_id -> state g → public_info → group_message
+val remove: #g:group_id -> state g → participant_id → group_message
 
 val update: #g:group_id -> state g → entropy → group_message
 
 // To send application data
 val send: #g:group_id -> state g → entropy → bytes → state g & group_message
 
-val process_welcome_message: welcome_message → (g:group_id & state g)
+// The application maintains a local store that maps the hash of a key package
+// to the corresponding private key.
+let key_callback = bytes -> option private_key
+
+// The application provides a callback to retrieve the private key associated to
+// a key package previously generated with `fresh_key_package`.
+val process_welcome_message: welcome_message → (lookup: key_callback) -> (g:group_id & state g)
+
 val process_group_message: #g:group_id -> state g → group_message → (state g & option bytes)
